x86/Archi.v
@@ -15,23 +15,20 @@
 (*                                                                     *)
 (* *********************************************************************)
 
-(** Architecture-dependent parameters for x86 in 32-bit mode *)
+(** Architecture-dependent parameters for x86 in 64-bit mode *)
 
 From Coq Require Import List ZArith.
 From Flocq Require Import Binary Bits.
 
-Definition ptr64 := false.
+Definition ptr64 := true.
 
 Definition big_endian := false.
 
-Definition align_int64 := 4%Z.
-Definition align_float64 := 4%Z.
-
-Definition splitlong := negb ptr64.
+Definition splitlong := false.
 
 Lemma splitlong_ptr32: splitlong = true -> ptr64 = false.
 Proof.
-  unfold splitlong. destruct ptr64; simpl; congruence.
+  unfold splitlong, ptr64; congruence.
 Qed.
 
 Definition default_nan_64 := (true, iter_nat 51 _ xO xH).
@@ -62,7 +59,7 @@ Definition float_of_single_preserves_sNaN := false.
 Definition float_conversion_default_nan := false.
 
 (** Which ABI to use. *)
-Parameter win64: bool.   (* Always false in 32 bits *)
+Parameter win64: bool.
 
 Global Opaque ptr64 big_endian splitlong
               default_nan_64 choose_nan_64
